Better norm control in tactics

src/lowparse/LowParse.SLow.Tac.Sum.fst
@@ -14,23 +14,83 @@ let rec enum_destr_tac'
   (ifc: if_combinator t eq)
   (u: unit { r_reflexive _ eq /\ r_transitive _ eq } )
   (#key #repr: eqtype)
-  (e: enum key repr { Cons? e } )
+  (e: enum key repr)
+  (eu: unit { Cons? e } )
+  (et: T.term) // implicit invariant: et represents e
 : T.Tac T.term
 = match e with
   | [_] ->
-    quote (enum_destr_cons_nil #key #repr #t eq e ())
+    let fu = quote (enum_destr_cons_nil #key #repr #t eq) in
+    T.mk_app fu [et, T.Q_Explicit]
   | _ ->
-    assert (Cons? e /\ Cons? (enum_tail e));
-    (fun (e_: enum key repr { Cons? e_ /\ Cons? (enum_tail e_) /\ e_ == e } ) ->
-      let (e' : enum key repr { Cons? e' } ) = enum_tail e_ in
-      let ar = enum_destr_tac' t eq ifc u e' in
-      let fu = quote (enum_destr_cons #key #repr #t eq ifc e ()) in
-      T.mk_app fu [ar, T.Q_Explicit]
+    assert (Cons? e /\ Cons? (enum_tail' e));
+    (fun (e_: enum key repr { Cons? e_ /\ Cons? (enum_tail' e_) /\ e_ == e } ) ->
+      let (e' : enum key repr { Cons? e' } ) = enum_tail' e_ in
+      let et'_fu = quote (enum_tail' #key #repr) in
+      let et' = T.mk_app et'_fu [et, T.Q_Explicit] in
+      let ar2 = enum_destr_tac' t eq ifc u e' () et' in
+      let fu = quote (enum_destr_cons #key #repr #t eq ifc) in
+      T.mk_app fu [
+        et, T.Q_Explicit;
+        ar2, T.Q_Explicit;
+      ]
     ) e
 
 (* Parser *)
 
-#set-options "--z3rlimit 64"
+#reset-options "--z3rlimit 128  --z3cliopt smt.arith.nl=false"
+
+noextract
+let parse32_sum_tac_ar2
+  (#kt: parser_kind)
+  (t: sum)
+  (#p: parser kt (sum_repr_type t))
+  (p32: parser32 p)
+  (#k: parser_kind)
+  (#pc: ((x: sum_key t) -> Tot (parser k (sum_cases t x))))
+  (pc32: ((x: sum_key t) -> Tot (parser32 (pc x))))
+  (#k' : parser_kind)
+  (#t' : Type0)
+  (p' : parser k' t')
+  (u: unit {
+    Cons? (sum_enum t) /\
+    k' == and_then_kind (parse_filter_kind kt) k /\
+    t' == sum_type t /\
+    p' == parse_sum t p pc
+  })
+: T.Tac T.term
+= let eq = feq bytes32 (option (sum_type t * U32.t)) (eq2 #_) in
+  let (eq_refl : unit { r_reflexive _ eq /\ r_transitive _ eq } ) = () in
+  let et = quote (sum_enum t) in
+  enum_destr_tac'
+      (bytes32 -> Tot (option (sum_type t * U32.t)))
+      (feq bytes32 (option (sum_type t * U32.t)) (eq2 #_))
+      (fif _ _ (eq2 #_) (default_if _))
+      eq_refl
+      (sum_enum t)
+      ()
+      et
+
+noextract
+let parse32_sum_tac_ar1
+  (#kt: parser_kind)
+  (t: sum)
+  (#p: parser kt (sum_repr_type t))
+  (p32: parser32 p)
+  (#k: parser_kind)
+  (#pc: ((x: sum_key t) -> Tot (parser k (sum_cases t x))))
+  (pc32: ((x: sum_key t) -> Tot (parser32 (pc x))))
+  (#k' : parser_kind)
+  (#t' : Type0)
+  (p' : parser k' t')
+  (u: unit {
+    Cons? (sum_enum t) /\
+    k' == and_then_kind (parse_filter_kind kt) k /\
+    t' == sum_type t /\
+    p' == parse_sum t p pc
+  })
+: T.Tac T.term
+= parse32_enum_key_tac' p32 (sum_enum t) () (parse_enum_key p (sum_enum t)) ()
 
 noextract
 let parse32_sum_tac'
@@ -51,18 +111,9 @@ let parse32_sum_tac'
     p' == parse_sum t p pc
   })
 : T.Tac T.term
-= let eq = feq bytes32 (option (sum_type t * U32.t)) (eq2 #_) in
-  let (eq_refl : unit { r_reflexive _ eq /\ r_transitive _ eq } ) = () in
-  let ar1 = parse32_enum_key_tac' p32 (sum_enum t) (parse_enum_key p (sum_enum t)) () in
-  let ar2 =
-    enum_destr_tac'
-      (bytes32 -> Tot (option (sum_type t * U32.t)))
-      (feq bytes32 (option (sum_type t * U32.t)) (eq2 #_))
-      (fif _ _ (eq2 #_) (default_if _))
-      eq_refl
-      (sum_enum t)
-  in
-  let fu = quote (
+= let ar1 : T.term = parse32_sum_tac_ar1 t p32 pc32 p' u in
+  let ar2 : T.term = parse32_sum_tac_ar2 t p32 pc32 p' u in
+  let fu : T.term = quote (
     parse32_sum_gen
       #kt
       t
@@ -76,10 +127,13 @@ let parse32_sum_tac'
       u
   )
   in
-  T.mk_app fu [
-    ar1, T.Q_Explicit;
-    ar2, T.Q_Explicit;
-  ]
+  let res : T.term = 
+    T.mk_app fu [
+      ar1, T.Q_Explicit;
+      ar2, T.Q_Explicit;
+    ]
+  in
+  res
 
 #reset-options
 
@@ -110,25 +164,40 @@ let parse32_sum_tac
 noextract
 let rec sum_destr_tac
   (v: Type)
-  (s: sum { Cons? (sum_enum s) } )
+  (s: sum)
+  (su: unit { Cons? (sum_enum s) } )
+  (st: T.term) // implicit invariant: st represents s
 : T.Tac T.term
   (decreases (sum_enum s))
 = let open T in
   match sum_enum s with
   | [_] ->
-    quote (sum_destr_cons_nil v s ())
+    let fu = quote (sum_destr_cons_nil v) in
+    T.mk_app fu [st, T.Q_Explicit]
   | _ ->
     let s' : sum = sum_tail s in
     assert (Cons? (sum_enum s')) ;
     let (s' : sum { Cons? (sum_enum s') } ) = s' in
-    let fu = quote (sum_destr_cons v s ()) in
-    let ar = sum_destr_tac v s' in
-    T.mk_app fu [ar, T.Q_Explicit]
+    let st'_fu = quote sum_tail in
+    let st' = T.mk_app st'_fu [st, T.Q_Explicit] in
+    let fu = quote (sum_destr_cons v) in
+    let ar2 = sum_destr_tac v s' () st' in
+    T.mk_app fu [
+      st, T.Q_Explicit;
+      ar2, T.Q_Explicit;
+    ]
+
+#set-options "--z3rlimit 32 "
+
+// assume val bidon_f (#t: Type) (x: t) : Tot unit
 
 noextract
-let serialize32_sum_tac'
+let serialize32_sum_tac_ar1
   (#kt: parser_kind)
-  (t: sum  { Cons? (sum_enum t) })
+  (t: sum)
+  (e: enum (sum_key_type t) (sum_repr_type t))
+//  (bidon: unit)
+  (tu: unit   { e == sum_enum t /\ Cons? e } )
   (#p: parser kt (sum_repr_type t))
   (#s: serializer p )
   (s32: serializer32 s)
@@ -149,8 +218,11 @@ let serialize32_sum_tac'
     s' == serialize_sum t s sc
   })
 : T.Tac T.term
-= let (e: enum (sum_key_type t) (sum_repr_type t) { Cons? e } ) = sum_enum t in
-  let ar1 = serialize32_enum_key_gen_tac'
+= let te = quote e in
+  T.print (T.term_to_string te);
+//  let tbidon = quote bidon in
+//  T.print (T.term_to_string tbidon);
+  serialize32_enum_key_gen_tac'
     #kt
     #(sum_key_type t)
     #(sum_repr_type t)
@@ -158,12 +230,42 @@ let serialize32_sum_tac'
     #s
     s32
     e
+    tu
     #(parse_filter_kind kt)
     #(parse_enum_key p e)
     (serialize_enum_key p s e)
     ()
-  in
-  let ar2 = sum_destr_tac bytes32 t in
+
+#set-options "--z3rlimit 128"
+
+noextract
+let serialize32_sum_tac'
+  (#kt: parser_kind)
+  (t: sum)
+  (tu: unit   { Cons? (sum_enum t) } )
+  (#p: parser kt (sum_repr_type t))
+  (#s: serializer p )
+  (s32: serializer32 s)
+  (#k: parser_kind)
+  (#pc: ((x: sum_key t) -> Tot (parser k (sum_cases t x))))
+  (#sc: ((x: sum_key t) -> Tot (serializer (pc x))))
+  (sc32: ((x: sum_key t) -> Tot (serializer32 (sc x))))
+  (u: unit { serializer32_sum_gen_precond kt k } )
+  (tag_of_data: ((x: sum_type t) -> Tot (y: sum_key_type t { y == sum_tag_of_data t x} )))
+  (#k' : parser_kind)
+  (#t' : Type0)
+  (#p' : parser k' t')
+  (s' : serializer p')
+  (u' : unit {
+    k' == and_then_kind (parse_filter_kind kt) k /\
+    t' == sum_type t /\
+    p' == parse_sum t p pc /\
+    s' == serialize_sum t s sc
+  })
+: T.Tac T.term
+= let st = quote t in
+  let ar1 = serialize32_sum_tac_ar1 #kt t (sum_enum t) (* bidon_f (sum_enum t) *) () #p #s s32 #k #pc #sc sc32 u tag_of_data #k'  #t'  #p' s' u' in
+  let ar2 = sum_destr_tac bytes32 t tu st in
   let fu = quote (
     serialize32_sum_gen
       #kt
@@ -183,14 +285,18 @@ let serialize32_sum_tac'
       u'
   )
   in
-  T.mk_app fu [
+  let res = T.mk_app fu [
     ar1, T.Q_Explicit;
     ar2, T.Q_Explicit;
   ]
+  in
+  res
+
+#set-options "--z3rlimit 32 "
 
 let serialize32_sum_tac_precond
   (#kt: parser_kind)
-  (t: sum  { Cons? (sum_enum t) })
+  (t: sum)
   (#p: parser kt (sum_repr_type t))
   (#s: serializer p )
   (s32: serializer32 s)
@@ -204,7 +310,8 @@ let serialize32_sum_tac_precond
   (#p' : parser k' t')
   (s' : serializer p')
 : GTot Type0
-=   k' == and_then_kind (parse_filter_kind kt) k /\
+=   Cons? (sum_enum t) /\
+    k' == and_then_kind (parse_filter_kind kt) k /\
     t' == sum_type t /\
     p' == parse_sum t p pc /\
     s' == serialize_sum t s sc
@@ -212,7 +319,7 @@ let serialize32_sum_tac_precond
 noextract
 let serialize32_sum_tac
   (#kt: parser_kind)
-  (t: sum  { Cons? (sum_enum t) })
+  (t: sum)
   (#p: parser kt (sum_repr_type t))
   (#s: serializer p )
   (s32: serializer32 s)
@@ -231,14 +338,17 @@ let serialize32_sum_tac
   })
   ()
 : T.Tac unit
-= let f = serialize32_sum_tac' #kt t #p #s s32 #k #pc #sc sc32 u tag_of_data s' u' in
+= let f = serialize32_sum_tac' #kt t () #p #s s32 #k #pc #sc sc32 u tag_of_data s' u' in
   T.print (T.term_to_string f);
   T.exact_guard f
+
+#set-options "--z3rlimit 64 "
 
 noextract
 let size32_sum_tac'
   (#kt: parser_kind)
-  (t: sum  { Cons? (sum_enum t) })
+  (t: sum)
+  (tu: unit { Cons? (sum_enum t) } )
   (#p: parser kt (sum_repr_type t))
   (#s: serializer p )
   (s32: size32 (serialize_enum_key _ s (sum_enum t)))
@@ -259,8 +369,8 @@ let size32_sum_tac'
     s' == serialize_sum t s sc
   })
 : T.Tac T.term
-= let (e: enum (sum_key_type t) (sum_repr_type t) { Cons? e } ) = sum_enum t in
-  let ar2 = sum_destr_tac U32.t t in
+= let st = quote t in
+  let ar2 = sum_destr_tac U32.t t tu st in
   let fu = quote (
     size32_sum_gen
       #kt
