src/lowparse/LowParse.SLow.Tac.Enum.fst
@@ -6,19 +6,29 @@ module T = FStar.Tactics
 noextract
 let rec maybe_enum_key_of_repr_tac'
   (#key #repr: eqtype)
-  (e: enum key repr { Cons? e } )
+  (e: enum key repr)
+  (u: unit { Cons? e } )
+  (et: T.term) // implicit invariant: et represents e
 : T.Tac T.term
   (decreases e)
 = match e with
   | [_] ->
-    quote (maybe_enum_key_of_repr'_t_cons_nil e ())
+    let fu = quote (maybe_enum_key_of_repr'_t_cons_nil #key #repr) in
+    T.mk_app fu [
+      et, T.Q_Explicit;
+    ]
   |  _ ->
-    assert (Cons? e /\ Cons? (enum_tail e));
-    (fun (e_ : enum key repr { Cons? e_ /\ Cons? (enum_tail e_) /\ e_ == e } ) ->
-      let (e' : enum key repr { Cons? e' } ) = enum_tail e_ in
-      let ar = maybe_enum_key_of_repr_tac' e' in
-      let fu = quote (maybe_enum_key_of_repr'_t_cons #key #repr e_ ()) in
-      (T.mk_app fu [ ar, T.Q_Explicit ])
+    assert (Cons? e /\ Cons? (enum_tail' e));
+    (fun (e_ : enum key repr { Cons? e_ /\ Cons? (enum_tail' e_) /\ e_ == e } ) ->
+      let (e' : enum key repr { Cons? e' } ) = enum_tail' e_ in
+      let et'_fu = quote (enum_tail' #key #repr) in
+      let et' = T.mk_app et'_fu [et, T.Q_Explicit] in
+      let ar2 = maybe_enum_key_of_repr_tac' e' () et' in
+      let fu = quote (maybe_enum_key_of_repr'_t_cons #key #repr) in
+      (T.mk_app fu [
+        et, T.Q_Explicit;
+        ar2, T.Q_Explicit;
+      ])
     ) e
 
 noextract
@@ -27,25 +37,34 @@ let maybe_enum_key_of_repr_tac
   (e: enum key repr { Cons? e } )
   ()
 : T.Tac unit
-= let g = maybe_enum_key_of_repr_tac' e in
+= let et = quote e in
+  let g = maybe_enum_key_of_repr_tac' e () et in
   T.print (T.term_to_string g) ;
   T.exact_guard g
 
 noextract
 let rec enum_repr_of_key_tac'
   (#key #repr: eqtype)
-  (e: enum key repr { Cons? e } )
+  (e: enum key repr)
+  (u: unit  { Cons? e } )
+  (et: T.term) // implicit invariant: et represents e
 : T.Tac T.term
 = match e with
   | [_] ->
-    quote (enum_repr_of_key_cons_nil e ())
+    let fu = quote (enum_repr_of_key_cons_nil #key #repr) in
+    T.mk_app fu [et, T.Q_Explicit]
   | (k, r) :: e' ->
     assert (Cons? e);
-    (fun (e_ : enum key repr { Cons? e_ /\ Cons? (enum_tail e_) /\ e_ == e } ) ->
-      let (e' : enum key repr { Cons? e' } ) = enum_tail e_ in
-      let ar = enum_repr_of_key_tac' e' in
-      let fu = quote (enum_repr_of_key_cons #key #repr e_ ()) in
-      T.mk_app fu [ ar, T.Q_Explicit ]
+    (fun (e_ : enum key repr { Cons? e_ /\ Cons? (enum_tail' e_) /\ e_ == e } ) ->
+      let (e' : enum key repr { Cons? e' } ) = enum_tail' e_ in
+      let et'_fu = quote (enum_tail' #key #repr) in
+      let et' = T.mk_app et'_fu [et, T.Q_Explicit] in
+      let ar2 = enum_repr_of_key_tac' e' () et' in
+      let fu = quote (enum_repr_of_key_cons #key #repr) in
+      T.mk_app fu [
+        et, T.Q_Explicit;
+        ar2, T.Q_Explicit;
+      ]
     ) e
 
 noextract
@@ -54,7 +73,8 @@ let enum_repr_of_key_tac
   (e: enum key repr { Cons? e } )
   ()
 : T.Tac unit
-= let g = enum_repr_of_key_tac' e in
+= let et = quote e in
+  let g = enum_repr_of_key_tac' e () et in
   T.exact_guard g
 
 noextract
@@ -63,7 +83,8 @@ let parse32_maybe_enum_key_tac'
   (#key #repr: eqtype)
   (#p: parser k repr)
   (p32: parser32 p)
-  (e: enum key repr { Cons? e } )
+  (e: enum key repr)
+  (eu: unit { Cons? e } )
   (#k' : parser_kind)
   (p' : parser k' (maybe_enum_key e))
   (u: unit {
@@ -71,7 +92,8 @@ let parse32_maybe_enum_key_tac'
     p' == parse_maybe_enum_key p e
   })
 : T.Tac T.term
-= let ar = maybe_enum_key_of_repr_tac' e in
+= let et = quote e in
+  let ar = maybe_enum_key_of_repr_tac' #key #repr e eu et in
   let fu = quote (parse32_maybe_enum_key_gen #k #key #repr #p p32 e #k' p' u) in
   T.mk_app fu [ar, T.Q_Explicit]
 
@@ -90,7 +112,7 @@ let parse32_maybe_enum_key_tac
   })
   ()
 : T.Tac unit
-= let f = parse32_maybe_enum_key_tac' p32 e p' u in
+= let f = parse32_maybe_enum_key_tac' p32 e () p' u in
   T.exact_guard f
 
 noextract
@@ -99,7 +121,8 @@ let parse32_enum_key_tac'
   (#key #repr: eqtype)
   (#p: parser k repr)
   (p32: parser32 p)
-  (e: enum key repr { Cons? e } )
+  (e: enum key repr)
+  (eu: unit { Cons? e } )
   (#k' : parser_kind)
   (p' : parser k' (enum_key e))
   (u: unit {
@@ -107,7 +130,7 @@ let parse32_enum_key_tac'
     p' == parse_enum_key p e
   })
 : T.Tac T.term
-= let ar = parse32_maybe_enum_key_tac' p32 e (parse_maybe_enum_key p e) () in
+= let ar = parse32_maybe_enum_key_tac' p32 e eu (parse_maybe_enum_key p e) () in
   let fu = quote (parse32_enum_key_gen #k #key #repr p e #k' p' u) in
   T.mk_app fu [ar, T.Q_Explicit]
 
@@ -126,7 +149,7 @@ let parse32_enum_key_tac
   })
   ()
 : T.Tac unit
-= let f = parse32_enum_key_tac' p32 e p' u in
+= let f = parse32_enum_key_tac' p32 e () p' u in
   T.exact_guard f
 
 noextract
@@ -136,7 +159,8 @@ let serialize32_enum_key_gen_tac'
   (#p: parser k repr)
   (#s: serializer p)
   (s32: serializer32 s)
-  (e: enum key repr { Cons? e } )
+  (e: enum key repr)
+  (eu: unit { Cons? e })
   (#k' : parser_kind)
   (#p' : parser k' (enum_key e))
   (s' : serializer p')
@@ -146,7 +170,9 @@ let serialize32_enum_key_gen_tac'
     s' == serialize_enum_key p s e
   })
 : T.Tac T.term
-= let ar = enum_repr_of_key_tac' e in
+= let et = quote e in
+  T.print (T.term_to_string et);
+  let ar = enum_repr_of_key_tac' e eu et in
   let fu = quote (serialize32_enum_key_gen #k #key #repr #p #s s32 e #k' #p' s' u) in
   T.mk_app fu [ar, T.Q_Explicit]
 
@@ -168,7 +194,7 @@ let serialize32_enum_key_gen_tac
   })
   ()
 : T.Tac unit
-= let f = serialize32_enum_key_gen_tac' s32 e s' u in
+= let f = serialize32_enum_key_gen_tac' s32 e () s' u in
   T.exact_guard f
 
 noextract
@@ -178,7 +204,8 @@ let serialize32_maybe_enum_key_tac'
   (#p: parser k repr)
   (#s: serializer p)
   (s32: serializer32 s)
-  (e: enum key repr { Cons? e } )
+  (e: enum key repr)
+  (eu: unit { Cons? e } )
   (#k' : parser_kind)
   (#p' : parser k' (maybe_enum_key e))
   (s' : serializer p')
@@ -188,7 +215,8 @@ let serialize32_maybe_enum_key_tac'
     s' == serialize_maybe_enum_key p s e
   })
 : T.Tac T.term
-= let ar = enum_repr_of_key_tac' e in
+= let et = quote e in
+  let ar = enum_repr_of_key_tac' e eu et in
   let fu = quote (serialize32_maybe_enum_key_gen #k #key #repr #p #s s32 e #k' #p' s' u) in
   T.mk_app fu [ar, T.Q_Explicit]
 
@@ -210,5 +238,5 @@ let serialize32_maybe_enum_key_tac
   })
   ()
 : T.Tac unit
-= let f = serialize32_maybe_enum_key_tac' s32 e s' u in
+= let f = serialize32_maybe_enum_key_tac' s32 e () s' u in
   T.exact_guard f
